Linglib.lean
@@ -67,6 +67,7 @@ import Linglib.Core.Computability.ContextFreeGrammar.Pumping
 import Linglib.Core.Computability.ContextFreeGrammar.Tree
 import Linglib.Core.Computability.ContextFreeGrammar.Weighted
 import Linglib.Core.Computability.Lens
+import Linglib.Core.Computability.Mealy
 import Linglib.Core.Computability.NonContextFree.AmBnCmDn
 import Linglib.Core.Computability.NonContextFree.AnBnCn
 import Linglib.Core.Computability.NonContextFree.AnBnCnDn
